Generalization of the initial rule for the dyadic system

FOLL/Syntax.v
@@ -30,7 +30,9 @@ Section LLSyntax.
   | Quest : oo -> oo 
   | All : (expr con -> oo) -> oo 
   | Some : (expr con -> oo) -> oo.
-  
+
+
+   
   (** Complexity of formulas *)
   Fixpoint complexity (X:oo) :=
     match X with
@@ -87,14 +89,14 @@ Section LLSyntax.
     | All X => Some (fun x => dual (X x))
     end.
 
-  (** Negation is involutive *)
+
+ 
+ (** Negation is involutive *)
   Theorem ng_involutive: forall F: oo, F = dual (dual F).
   Proof.
     intro. 
     induction F; simpl; auto;
       try( try(rewrite <- IHF1); try(rewrite <- IHF2); try(rewrite <- IHF);auto);
-     
-      
       try(assert (o = fun x =>  dual (dual (o x))) by
              (extensionality e; apply H); rewrite <- H0; auto).
   Qed.
@@ -156,12 +158,60 @@ Qed.
     induction H;subst;simpl;firstorder.
   Qed.
 
+ (** Well formedness condition  *)
+  Inductive isFormula: oo -> Prop  :=
+  | wf_atm : forall (P1:atm), isFormula (atom P1)
+  | wf_perp : forall (P1:atm), isFormula (perp P1)
+  | wf_Top : isFormula Top
+  | wf_One : isFormula One
+  | wf_Zero : isFormula Zero
+  | wf_Bot : isFormula Bot
+  | wf_AAnd : forall (A1 A2 :oo), isFormula A1  -> isFormula A2  -> isFormula (AAnd A1 A2)
+  | wf_MAnd : forall (A1 A2 :oo), isFormula A1  -> isFormula A2  -> isFormula (MAnd A1 A2)
+  | wf_AOr : forall (A1 A2 :oo), isFormula A1  -> isFormula A2  -> isFormula (AOr A1 A2)
+  | wf_MOr : forall (A1 A2 :oo), isFormula A1  -> isFormula A2  -> isFormula (MOr A1 A2)
+  | wf_Bang : forall (A1 :oo), isFormula A1 -> isFormula (Bang A1)
+  | wf_Quest : forall (A1 :oo), isFormula A1 -> isFormula (Quest A1)
+  | wf_All : forall (A : expr con -> oo), uniform_oo A -> (forall t: expr con, isFormula (A t)) -> isFormula (All A)
+  | wf_Some : forall (A : expr con -> oo), uniform_oo A -> (forall t: expr con, isFormula (A t)) -> isFormula (Some A).
+  
+  (** Well formendness conditions for lists and arrows *)
+  Definition isFormulaL  (L:list oo)  := Forall isFormula L. 
+ 
+  Lemma isFormulaIn F L: 
+      isFormulaL L -> In F L -> isFormula F. 
+  Proof.
+    intros.
+    eapply @ForallIn with (F:=F) in H;auto.
+  Qed.
+
+
+Lemma isFormulaInP F L L': 
+      isFormulaL L -> Permutation L (F::L') -> isFormula F. 
+  Proof.
+ intros.
+    eapply @ForallInP with (F:=F) in H;auto.
+  Qed.
+ 
+ 
+  Generalizable All Variables.
+  Global Instance isFormulaL_morph : 
+    Proper ((@Permutation oo) ==> Basics.impl) (isFormulaL).
+  Proof.
+    unfold Proper; unfold respectful; unfold Basics.impl.
+    intros.
+    unfold isFormulaL.
+    rewrite <- H;auto.
+  Qed.  
+
  
 End LLSyntax.
 
-Global Hint Constructors uniform_oo : core.
+Global Hint Constructors uniform_oo isFormula: core.
 Global Hint Resolve Complexity0
                     DualComplexity: core.
+
+Global Hint Unfold isFormulaL :core.
 
 Module LLNotations .
   Notation "'⊥'" := Bot.
